split ml_copying_gc, also general progress

x86-64/ml_copying_gcScript.sml
@@ -188,7 +188,7 @@ val gc_inv_def = Define `
 
 (* Invariant maintained *)
 
-val heap_lookup_MEM = prove(
+val heap_lookup_MEM = store_thm("heap_lookup_MEM",
   ``!heap n x. (heap_lookup n heap = SOME x) ==> MEM x heap``,
   Induct \\ FULL_SIMP_TAC std_ss [heap_lookup_def] \\ SRW_TAC [] []
   \\ RES_TAC \\ FULL_SIMP_TAC std_ss []);
@@ -261,11 +261,11 @@ val isSomeDataOrForward_lemma = prove(
   \\ SRW_TAC [] [] \\ FULL_SIMP_TAC std_ss []
   \\ EVAL_TAC \\ FULL_SIMP_TAC std_ss [el_length_def]);
 
-val FILTER_APPEND = prove(
+val FILTER_APPEND = store_thm("FILTER_APPEND",
   ``!xs ys p. FILTER p (xs ++ ys) = FILTER p xs ++ FILTER p ys``,
   Induct \\ SRW_TAC [] [FILTER]);
 
-val EVERY2_SPLIT = prove(
+val EVERY2_SPLIT = store_thm("EVERY2_SPLIT",
   ``!xs1 zs.
       EVERY2 P zs (xs1 ++ x::xs2) ==>
       ?ys1 y ys2. (zs = ys1 ++ y::ys2) /\ EVERY2 P ys1 xs1 /\
@@ -276,7 +276,7 @@ val EVERY2_SPLIT = prove(
   THEN1 (REPEAT STRIP_TAC \\ Q.LIST_EXISTS_TAC [`[]`,`h`,`t`] \\ SRW_TAC [] [])
   \\ Q.LIST_EXISTS_TAC [`h::ys1`,`y`,`ys2`] \\ FULL_SIMP_TAC (srw_ss()) []);
 
-val EVERY2_SPLIT_ALT = prove(
+val EVERY2_SPLIT_ALT = store_thm("EVERY2_SPLIT_ALT",
   ``!xs1 zs.
       EVERY2 P (xs1 ++ x::xs2) zs ==>
       ?ys1 y ys2. (zs = ys1 ++ y::ys2) /\ EVERY2 P xs1 ys1 /\
@@ -287,13 +287,13 @@ val EVERY2_SPLIT_ALT = prove(
   THEN1 (Q.LIST_EXISTS_TAC [`[]`] \\ FULL_SIMP_TAC (srw_ss()) [])
   \\ Q.LIST_EXISTS_TAC [`h::ys1`,`y`,`ys2`] \\ FULL_SIMP_TAC (srw_ss()) []);
 
-val EVERY2_APPEND = prove(
+val EVERY2_APPEND = store_thm("EVERY2_APPEND",
   ``!xs ts.
       (LENGTH xs = LENGTH ts) ==>
       (EVERY2 P (xs ++ ys) (ts ++ us) = EVERY2 P xs ts /\ EVERY2 P ys us)``,
   Induct \\ Cases_on `ts` \\ FULL_SIMP_TAC (srw_ss()) [LENGTH,CONJ_ASSOC]);
 
-val EVERY2_IMP_LENGTH = prove(
+val EVERY2_IMP_LENGTH = store_thm("EVERY2_IMP_LENGTH",
   ``!xs ys. EVERY2 P xs ys ==> (LENGTH xs = LENGTH ys)``,
   Induct \\ Cases_on `ys` \\ FULL_SIMP_TAC (srw_ss()) [LENGTH,CONJ_ASSOC]);
 
@@ -350,19 +350,19 @@ val BIJ_UPDATE = prove(
   SIMP_TAC std_ss [BIJ_DEF,SURJ_DEF,INJ_DEF,IN_INSERT,APPLY_UPDATE_THM]
   \\ METIS_TAC []);
 
-val INJ_UPDATE = prove(
+val INJ_UPDATE = store_thm("INJ_UPDATE",
   ``INJ f s t /\ ~(x IN s) /\ ~(y IN t) ==>
     INJ ((x =+ y) f) (x INSERT s) (y INSERT t)``,
   SIMP_TAC std_ss [BIJ_DEF,SURJ_DEF,INJ_DEF,IN_INSERT,APPLY_UPDATE_THM]
   \\ METIS_TAC []);
 
-val heap_lookup_PREFIX = prove(
+val heap_lookup_PREFIX = store_thm("heap_lookup_PREFIX",
   ``!xs. (heap_lookup (heap_length xs) (xs ++ x::ys) = SOME x)``,
   Induct \\ FULL_SIMP_TAC (srw_ss()) [heap_lookup_def,APPEND,heap_length_def]
   \\ SRW_TAC [] [] \\ Cases_on `h`
   \\ FULL_SIMP_TAC std_ss [el_length_def] \\ DECIDE_TAC);
 
-val heap_lookup_EXTEND = prove(
+val heap_lookup_EXTEND = store_thm("heap_lookup_EXTEND",
   ``!xs n ys x. (heap_lookup n xs = SOME x) ==>
                 (heap_lookup n (xs ++ ys) = SOME x)``,
   Induct \\ FULL_SIMP_TAC (srw_ss()) [heap_lookup_def] \\ SRW_TAC [] []);
@@ -540,7 +540,8 @@ val gc_move_list_APPEND_lemma = prove(
   \\ CONV_TAC (DEPTH_CONV PairRules.PBETA_CONV)
   \\ FULL_SIMP_TAC std_ss [APPEND_ASSOC] \\ METIS_TAC []);
 
-val IMP_IMP = METIS_PROVE [] ``b /\ (b1 ==> b2) ==> (b ==> b1) ==> b2``
+val IMP_IMP = save_thm("IMP_IMP",
+  METIS_PROVE [] ``b /\ (b1 ==> b2) ==> (b ==> b1) ==> b2``);
 
 val heap_addresses_APPEND = prove(
   ``!xs ys n. heap_addresses n (xs ++ ys) =
@@ -548,13 +549,13 @@ val heap_addresses_APPEND = prove(
   Induct \\ FULL_SIMP_TAC (srw_ss()) [APPEND,heap_addresses_def,heap_length_def]
   \\ FULL_SIMP_TAC (srw_ss()) [EXTENSION,DISJ_ASSOC,ADD_ASSOC]);
 
-val LESS_IMP_heap_lookup = prove(
+val LESS_IMP_heap_lookup = store_thm("LESS_IMP_heap_lookup",
   ``!xs j ys. j < heap_length xs ==> (heap_lookup j (xs ++ ys) = heap_lookup j xs)``,
   Induct \\ FULL_SIMP_TAC (srw_ss()) [heap_length_def,heap_lookup_def]
   \\ SRW_TAC [] [] \\ `j - el_length h < SUM (MAP el_length xs)` by DECIDE_TAC
   \\ FULL_SIMP_TAC std_ss []);
 
-val NOT_LESS_IMP_heap_lookup = prove(
+val NOT_LESS_IMP_heap_lookup = store_thm("NOT_LESS_IMP_heap_lookup",
   ``!xs j ys. ~(j < heap_length xs) ==>
               (heap_lookup j (xs ++ ys) = heap_lookup (j - heap_length xs) ys)``,
   Induct \\ FULL_SIMP_TAC (srw_ss()) [heap_length_def,heap_lookup_def]
@@ -675,7 +676,7 @@ val gc_inv_init = prove(
   \\ FULL_SIMP_TAC (srw_ss()) [heaps_similar_REFL,heap_map_EMPTY,FLOOKUP_DEF]
   \\ FULL_SIMP_TAC (srw_ss()) [BIJ_DEF,INJ_DEF,SURJ_DEF]);
 
-val full_gc_thm = prove(
+val full_gc_thm = store_thm("full_gc_thm",
   ``roots_ok roots heap /\ heap_ok (heap:('a,'b) heap_element list) limit ==>
     ?heap2 a2 heap3.
       (full_gc (roots:'a heap_address list,heap,limit) =
@@ -709,7 +710,7 @@ val MEM_ADDR_MAP = prove(
   Induct \\ TRY (Cases_on `h`) \\ FULL_SIMP_TAC (srw_ss()) [ADDR_MAP_def]
   \\ REPEAT STRIP_TAC \\ FULL_SIMP_TAC std_ss [] \\ RES_TAC \\ METIS_TAC []);
 
-val heap_length_heap_expand = prove(
+val heap_length_heap_expand = store_thm("heap_length_heap_expand",
   ``!n. heap_length (heap_expand n) = n``,
   Cases \\ EVAL_TAC \\ FULL_SIMP_TAC (srw_ss()) [el_length_def,ADD1]);
 
@@ -718,7 +719,7 @@ val EVERY_isDataElement_IMP_LEMMA = prove(
   Induct \\ FULL_SIMP_TAC (srw_ss()) [isDataElement_def] \\ REPEAT STRIP_TAC
   \\ FULL_SIMP_TAC (srw_ss()) [isForwardPointer_def]);
 
-val heap_lookup_LESS = prove(
+val heap_lookup_LESS = store_thm("heap_lookup_LESS",
   ``!xs n. (heap_lookup n xs = SOME x) ==> n < heap_length xs``,
   Induct \\ FULL_SIMP_TAC std_ss [heap_lookup_def] \\ SRW_TAC [] []
   \\ RES_TAC \\ Cases_on `h` \\ FULL_SIMP_TAC (srw_ss())
@@ -731,7 +732,7 @@ val isSome_heap_looukp_IMP_APPEND = prove(
   \\ IMP_RES_TAC heap_lookup_LESS \\ IMP_RES_TAC LESS_IMP_heap_lookup
   \\ FULL_SIMP_TAC (srw_ss()) []);
 
-val MEM_IMP_heap_lookup = prove(
+val MEM_IMP_heap_lookup = store_thm("MEM_IMP_heap_lookup",
   ``!xs x. MEM x xs ==> ?j. (heap_lookup j xs = SOME x)``,
   Induct \\ FULL_SIMP_TAC std_ss [MEM,heap_lookup_def,heap_addresses_def]
   \\ SRW_TAC [] [] \\ RES_TAC THEN1 METIS_TAC []
@@ -746,7 +747,7 @@ val heap_lookup_IMP_heap_addresses = prove(
   \\ `n + el_length h + (j - el_length h) = n + j` by DECIDE_TAC
   \\ METIS_TAC []) |> Q.SPECL [`xs`,`0`] |> SIMP_RULE std_ss [] |> GEN_ALL;
 
-val full_gc_LENGTH = prove(
+val full_gc_LENGTH = store_thm("full_gc_LENGTH",
   ``roots_ok roots heap /\ heap_ok (heap:('a,'b) heap_element list) limit ==>
     ?roots2 heap2 a2.
       (full_gc (roots:'a heap_address list,heap,limit) =
@@ -754,7 +755,7 @@ val full_gc_LENGTH = prove(
   REPEAT STRIP_TAC \\ MP_TAC full_gc_thm \\ FULL_SIMP_TAC std_ss []
   \\ REPEAT STRIP_TAC \\ FULL_SIMP_TAC std_ss [gc_inv_def,APPEND_NIL]);
 
-val full_gc_ok = prove(
+val full_gc_ok = store_thm("full_gc_ok",
   ``roots_ok roots heap /\ heap_ok (heap:('a,'b) heap_element list) limit ==>
     ?roots2 heap2 a2.
       (full_gc (roots:'a heap_address list,heap,limit) = (roots2,heap2,a2,T)) /\
@@ -806,7 +807,7 @@ val gc_related_def = Define `
       (heap_lookup (f ' i) heap2 = SOME (DataElement (ADDR_MAP (FAPPLY f) xs) l d)) /\
       !ptr. MEM (Pointer ptr) xs ==> ptr IN FDOM f`;
 
-val full_gc_related = prove(
+val full_gc_related = store_thm("full_gc_related",
   ``roots_ok roots heap /\ heap_ok (heap:('a,'b) heap_element list) limit ==>
     ?heap2 a2 f.
       (full_gc (roots:'a heap_address list,heap,limit) =
@@ -834,455 +835,6 @@ val full_gc_related = prove(
   \\ RES_TAC \\ FULL_SIMP_TAC (srw_ss()) [APPEND_NIL]
   \\ IMP_RES_TAC heap_lookup_LESS \\ IMP_RES_TAC heap_lookup_EXTEND
   \\ FULL_SIMP_TAC std_ss []);
-
-(* refinement invariant *)
-
-val small_int_def = Define `
-  small_int i = 0 <= i /\ (i:int) < & (2 ** 62)`;
-
-val mw_def = tDefine "mw" `
-  mw n = if n = 0 then []:'a word list else
-           n2w (n MOD dimword (:'a)) :: mw (n DIV dimword(:'a))`
-   (WF_REL_TAC `measure I`
-    \\ SIMP_TAC std_ss [MATCH_MP DIV_LT_X ZERO_LT_dimword,ONE_LT_dimword]
-    \\ DECIDE_TAC);
-
-val _ = Hol_datatype `tag = BlockTag of num | RefTag | NumTag of bool`;
-
-val DataOnly_def = Define `
-  DataOnly b xs = DataElement [] (LENGTH xs) (NumTag b,xs)`;
-
-val BlockRep_def = Define `
-  BlockRep tag xs = DataElement xs (LENGTH xs) (BlockTag tag,[])`;
-
-val bc_value_size_LEMMA = prove(
-  ``!vs v. MEM v vs ==> bc_value_size v <= bc_value1_size vs``,
-  Induct \\ FULL_SIMP_TAC (srw_ss()) [bc_value_size_def]
-  \\ REPEAT STRIP_TAC \\ RES_TAC \\ FULL_SIMP_TAC std_ss [] \\ DECIDE_TAC);
-
-val _ = type_abbrev("ml_el",``:('a word, tag # ('b word list)) heap_element``);
-val _ = type_abbrev("ml_heap",``:('a,'b) ml_el list``);
-
-val EVERY2_cong = store_thm("EVERY2_cong",
-  ``!l1 l1' l2 l2' P P'.
-      (l1 = l1') /\ (l2 = l2') /\
-      (!x y. MEM x l1' /\ MEM y l2' ==> (P x y = P' x y)) ==>
-      (EVERY2 P l1 l2 = EVERY2 P' l1' l2')``,
-  Induct \\ Cases_on `l2'` \\ SIMP_TAC (srw_ss()) [EVERY2_def] \\ METIS_TAC[])
-val _ = DefnBase.export_cong "EVERY2_cong"
-
-val bc_value_inv_def = tDefine "bc_value_inv" `
-  (bc_value_inv (Number i) (x,f,heap:('a,'b) ml_heap) =
-     if small_int i then (x = Data ((2w * n2w (Num i)):'a word)) else
-       ?ptr. (x = Pointer ptr) /\
-             (heap_lookup ptr heap =
-                SOME (DataOnly (i < 0) ((mw (Num (ABS i))):'b word list)))) /\
-  (bc_value_inv (CodePtr n) (x,f,heap) =
-     (x = Data (n2w n)) /\ n < dimword (:'a)) /\
-  (bc_value_inv (RefPtr n) (x,f,heap) =
-     (x = Pointer (f ' n)) /\ n IN FDOM f) /\
-  (bc_value_inv (Block n vs) (x,f,heap) =
-     if vs = [] then (x = Data ((2w * n2w n + 1w):'a word)) /\ (n < 2 ** 62) else
-       ?ptr xs.
-         EVERY2 (\v x. bc_value_inv v (x,f,heap)) vs xs /\
-         (x = Pointer ptr) /\
-         (heap_lookup ptr heap =
-            SOME (BlockRep n xs))) /\
-  (bc_value_inv (StackPtr n) (x,f,heap) = F)`
- (WF_REL_TAC `measure (bc_value_size o FST)` \\ REPEAT STRIP_TAC
-  \\ IMP_RES_TAC bc_value_size_LEMMA \\ DECIDE_TAC);
-
-val get_refs_def = tDefine "get_refs" `
-  (get_refs (Number _) = []) /\
-  (get_refs (CodePtr _) = []) /\
-  (get_refs (RefPtr p) = [p]) /\
-  (get_refs (Block tag vs) = FLAT (MAP get_refs vs))`
- (WF_REL_TAC `measure (bc_value_size)` \\ REPEAT STRIP_TAC \\ Induct_on `vs`
-  \\ SRW_TAC [] [bc_value_size_def] \\ RES_TAC \\ DECIDE_TAC);
-
-val ref_edge_def = Define `
-  ref_edge refs x y = x IN FDOM refs /\ MEM y (get_refs (refs ' x))`;
-
-val reachable_refs_def = Define `
-  reachable_refs roots refs t =
-    ?x r. MEM x roots /\ MEM r (get_refs x) /\ RTC (ref_edge refs) r t`;
-
-val RefBlock_def = Define `
-  RefBlock x = DataElement [x] 1 (RefTag,[])`;
-
-val bc_ref_inv_def = Define `
-  bc_ref_inv n refs (f,heap) =
-    n IN FDOM f /\ n IN FDOM refs /\
-    ?y. (heap_lookup (FAPPLY f n) heap = SOME (RefBlock y)) /\
-        bc_value_inv (FAPPLY refs n) (y,f,heap)`;
-
-val bc_stack_ref_inv_def = Define `
-  bc_stack_ref_inv stack (refs:num|->bc_value) (roots, heap) =
-    ?f. INJ (FAPPLY f) (FDOM f) { a | isSomeDataElement (heap_lookup a heap) } /\
-        FDOM f SUBSET FDOM refs /\
-        EVERY2 (\v x. bc_value_inv v (x,f,heap)) stack roots /\
-        !n. reachable_refs stack refs n ==> bc_ref_inv n refs (f,heap)`;
-
-val unused_space_inv_def = Define `
-  unused_space_inv ptr l heap =
-    l <> 0 ==> (heap_lookup ptr heap = SOME (Unused (l-1)))`;
-
-val abs_ml_inv_def = Define `
-  abs_ml_inv stack refs (roots,heap,a,sp) limit =
-    roots_ok roots heap /\ heap_ok heap limit /\
-    unused_space_inv a sp heap /\
-    bc_stack_ref_inv stack refs (roots,heap)`;
-
-(* Prove refinement is maintained past GC calls *)
-
-val LENGTH_ADDR_MAP = prove(
-  ``!xs f. LENGTH (ADDR_MAP f xs) = LENGTH xs``,
-  Induct \\ TRY (Cases_on `h`) \\ SRW_TAC [] [ADDR_MAP_def]);
-
-val PULL_EXISTS = METIS_PROVE [] ``(((?x. P x) ==> Q) = !x. P x ==> Q) /\
-                                   ((?x. P x) /\ Q = ?x. P x /\ Q)``
-
-val MEM_IMP_bc_value_size = prove(
-  ``!l a. MEM a l ==> bc_value_size a < 1 + bc_value1_size l``,
-  Induct \\ FULL_SIMP_TAC std_ss [MEM,bc_value_size_def]
-  \\ REPEAT STRIP_TAC \\ FULL_SIMP_TAC std_ss [] \\ RES_TAC \\ DECIDE_TAC);
-
-val EL_ADDR_MAP = prove(
-  ``!xs n f.
-      n < LENGTH xs ==> (EL n (ADDR_MAP f xs) = ADDR_APPLY f (EL n xs))``,
-  Induct \\ FULL_SIMP_TAC (srw_ss()) [] \\ Cases_on `n` \\ Cases_on `h`
-  \\ FULL_SIMP_TAC (srw_ss()) [ADDR_MAP_def,ADDR_APPLY_def]);
-
-val EVERY2_EVERY = prove(
-  ``!xs ys f.
-      EVERY2 f xs ys <=>
-      (LENGTH xs = LENGTH ys) /\ EVERY (UNCURRY f) (ZIP (xs,ys))``,
-  Induct \\ Cases_on `ys` \\ FULL_SIMP_TAC (srw_ss()) [] \\ METIS_TAC []);
-
-val bc_value_inv_related = prove(
-  ``!w x f.
-      gc_related g heap1 heap2 /\
-      (!ptr. (x = Pointer ptr) ==> ptr IN FDOM g) /\
-      bc_value_inv w (x,f,heap1) ==>
-      bc_value_inv w (ADDR_APPLY (FAPPLY g) x,g f_o_f f,heap2) /\
-      EVERY (\n. f ' n IN FDOM g) (get_refs w)``,
-  completeInduct_on `bc_value_size w` \\ NTAC 5 STRIP_TAC
-  \\ FULL_SIMP_TAC std_ss [PULL_FORALL] \\ Cases_on `w` THEN1
-   (FULL_SIMP_TAC std_ss [bc_value_inv_def,get_refs_def,EVERY_DEF]
-    \\ Cases_on `small_int i`
-    \\ FULL_SIMP_TAC (srw_ss()) [ADDR_APPLY_def,DataOnly_def]
-    \\ FULL_SIMP_TAC std_ss [gc_related_def] \\ RES_TAC
-    \\ FULL_SIMP_TAC std_ss [ADDR_MAP_def])
-  THEN1
-   (FULL_SIMP_TAC (srw_ss()) [bc_value_inv_def,ADDR_APPLY_def,BlockRep_def]
-    \\ Cases_on `l = []` \\ FULL_SIMP_TAC std_ss []
-    THEN1 (FULL_SIMP_TAC (srw_ss()) [get_refs_def,ADDR_APPLY_def])
-    \\ FULL_SIMP_TAC (srw_ss()) [bc_value_inv_def,ADDR_APPLY_def,BlockRep_def]
-    \\ FULL_SIMP_TAC std_ss [gc_related_def] \\ RES_TAC
-    \\ FULL_SIMP_TAC (srw_ss()) [] \\ NTAC 2 (POP_ASSUM MP_TAC)
-    \\ FULL_SIMP_TAC std_ss [LENGTH_ADDR_MAP] \\ STRIP_TAC
-    \\ REVERSE STRIP_TAC THEN1
-     (FULL_SIMP_TAC std_ss [get_refs_def,EVERY_MEM,MEM_FLAT,PULL_EXISTS,MEM_MAP]
-      \\ FULL_SIMP_TAC std_ss [bc_value_size_def] \\ REPEAT STRIP_TAC
-      \\ Q.MATCH_ASSUM_RENAME_TAC `MEM k (get_f a)` []
-      \\ IMP_RES_TAC MEM_IMP_bc_value_size
-      \\ `bc_value_size a < 1 + (n + bc_value1_size l)` by DECIDE_TAC
-      \\ `?l1 l2. l = l1 ++ a::l2` by METIS_TAC [MEM_SPLIT]
-      \\ FULL_SIMP_TAC std_ss [] \\ IMP_RES_TAC EVERY2_SPLIT_ALT
-      \\ FULL_SIMP_TAC std_ss [MEM_APPEND,MEM]
-      \\ RES_TAC \\ METIS_TAC [])
-    \\ FULL_SIMP_TAC std_ss [EVERY2_EVERY,LENGTH_ADDR_MAP,EVERY_MEM,FORALL_PROD]
-    \\ Q.PAT_ASSUM `LENGTH l = LENGTH xs` ASSUME_TAC
-    \\ FULL_SIMP_TAC std_ss [MEM_ZIP,LENGTH_ADDR_MAP,PULL_EXISTS]
-    \\ STRIP_TAC \\ STRIP_TAC
-    \\ Q.MATCH_ASSUM_RENAME_TAC `t < LENGTH xs` [] \\ RES_TAC
-    \\ `MEM (EL t l) l` by (FULL_SIMP_TAC std_ss [MEM_EL] \\ METIS_TAC [])
-    \\ `MEM (EL t xs) xs` by (FULL_SIMP_TAC std_ss [MEM_EL] \\ METIS_TAC [])
-    \\ `(!ptr. (EL t xs = Pointer ptr) ==> ptr IN FDOM g)` by METIS_TAC []
-    \\ `bc_value_size (EL t l)  < bc_value_size (Block n l)` by ALL_TAC THEN1
-     (FULL_SIMP_TAC std_ss [bc_value_size_def]
-      \\ IMP_RES_TAC MEM_IMP_bc_value_size \\ DECIDE_TAC)
-    \\ RES_TAC \\ FULL_SIMP_TAC std_ss [EL_ADDR_MAP])
-  THEN1
-    (FULL_SIMP_TAC (srw_ss()) [bc_value_inv_def,ADDR_APPLY_def,get_refs_def])
-  THEN1
-    (FULL_SIMP_TAC (srw_ss()) [bc_value_inv_def,ADDR_APPLY_def]
-     \\ `n IN FDOM (g f_o_f f)` by ALL_TAC \\ ASM_SIMP_TAC std_ss []
-     \\ FULL_SIMP_TAC (srw_ss()) [f_o_f_DEF,get_refs_def])
-  THEN1
-    (FULL_SIMP_TAC (srw_ss()) [bc_value_inv_def]));
-
-val bc_ref_inv_related = prove(
-  ``gc_related g heap1 heap2 /\
-    bc_ref_inv n refs (f,heap1) /\ (f ' n) IN FDOM g ==>
-    bc_ref_inv n refs (g f_o_f f,heap2)``,
-  FULL_SIMP_TAC std_ss [bc_ref_inv_def] \\ STRIP_TAC \\ FULL_SIMP_TAC std_ss []
-  \\ FULL_SIMP_TAC (srw_ss()) [f_o_f_DEF,gc_related_def,RefBlock_def] \\ RES_TAC
-  \\ FULL_SIMP_TAC (srw_ss()) [] \\ Q.EXISTS_TAC `ADDR_APPLY (FAPPLY g) y`
-  \\ STRIP_TAC
-  THEN1 (Cases_on `y` \\ FULL_SIMP_TAC std_ss [ADDR_MAP_def,ADDR_APPLY_def])
-  \\ `gc_related g heap1 heap2` by ALL_TAC
-  THEN1 (FULL_SIMP_TAC (srw_ss()) [gc_related_def] \\ METIS_TAC [])
-  \\ IMP_RES_TAC bc_value_inv_related \\ METIS_TAC []);
-
-val RTC_lemma = prove(
-  ``!r n. RTC (ref_edge refs) r n ==>
-          (!m. RTC (ref_edge refs) r m ==> bc_ref_inv m refs (f,heap)) /\
-          gc_related g heap heap2 /\
-          f ' r IN FDOM g ==> f ' n IN FDOM g``,
-  HO_MATCH_MP_TAC RTC_INDUCT \\ FULL_SIMP_TAC std_ss [] \\ REPEAT STRIP_TAC
-  \\ FULL_SIMP_TAC std_ss []
-  \\ Q.PAT_ASSUM `bb ==> bbb` MATCH_MP_TAC \\ FULL_SIMP_TAC std_ss []
-  \\ STRIP_TAC THEN1
-   (REPEAT STRIP_TAC \\ Q.PAT_ASSUM `!x.bb` MATCH_MP_TAC \\ METIS_TAC [RTC_CASES1])
-  \\ `RTC (ref_edge refs) r r' /\ RTC (ref_edge refs) r r` by METIS_TAC [RTC_CASES1]
-  \\ RES_TAC \\ Q.PAT_ASSUM `!x.bb` (K ALL_TAC)
-  \\ FULL_SIMP_TAC std_ss [bc_ref_inv_def,RefBlock_def]
-  \\ `!ptr. MEM (Pointer ptr) [y] ==> ptr IN FDOM g` by ALL_TAC
-  THEN1 (FULL_SIMP_TAC std_ss [gc_related_def] \\ RES_TAC)
-  \\ FULL_SIMP_TAC std_ss [MEM]
-  \\ POP_ASSUM (ASSUME_TAC o ONCE_REWRITE_RULE [EQ_SYM_EQ])
-  \\ `EVERY (\n. f ' n IN FDOM g) (get_refs (refs ' r))` by ALL_TAC
-  THEN1 (IMP_RES_TAC bc_value_inv_related)
-  \\ FULL_SIMP_TAC std_ss [ref_edge_def,EVERY_MEM]);
-
-val reachable_refs_lemma = prove(
-  ``gc_related g heap heap2 /\
-    EVERY2 (\v x. bc_value_inv v (x,f,heap)) stack roots /\
-    (!n. reachable_refs stack refs n ==> bc_ref_inv n refs (f,heap)) /\
-    (!ptr. MEM (Pointer ptr) roots ==> ptr IN FDOM g) ==>
-    (!n. reachable_refs stack refs n ==> n IN FDOM f /\ (f ' n) IN FDOM g)``,
-  NTAC 3 STRIP_TAC \\ FULL_SIMP_TAC std_ss [reachable_refs_def,PULL_EXISTS]
-  \\ `?xs1 xs2. stack = xs1 ++ x::xs2` by METIS_TAC [MEM_SPLIT]
-  \\ FULL_SIMP_TAC std_ss [] \\ IMP_RES_TAC EVERY2_SPLIT_ALT
-  \\ FULL_SIMP_TAC std_ss [MEM,MEM_APPEND]
-  \\ `EVERY (\n. f ' n IN FDOM g) (get_refs x)` by METIS_TAC [bc_value_inv_related]
-  \\ FULL_SIMP_TAC std_ss [EVERY_MEM] \\ RES_TAC \\ FULL_SIMP_TAC std_ss []
-  \\ `n IN FDOM f` by FULL_SIMP_TAC std_ss [bc_ref_inv_def]
-  \\ FULL_SIMP_TAC std_ss []
-  \\ `bc_ref_inv r refs (f,heap)` by METIS_TAC [RTC_REFL]
-  \\ `(!m. RTC (ref_edge refs) r m ==> bc_ref_inv m refs (f,heap))` by ALL_TAC
-  THEN1 METIS_TAC [] \\ IMP_RES_TAC RTC_lemma);
-
-val bc_stack_ref_inv_related = prove(
-  ``gc_related g heap1 heap2 /\
-    bc_stack_ref_inv stack refs (roots,heap1) /\
-    (!ptr. MEM (Pointer ptr) roots ==> ptr IN FDOM g) ==>
-    bc_stack_ref_inv stack refs (ADDR_MAP (FAPPLY g) roots,heap2)``,
-  REPEAT STRIP_TAC \\ FULL_SIMP_TAC std_ss [bc_stack_ref_inv_def]
-  \\ Q.EXISTS_TAC `g f_o_f f` \\ REPEAT STRIP_TAC
-  THEN1 (FULL_SIMP_TAC (srw_ss()) [INJ_DEF,gc_related_def,f_o_f_DEF])
-  THEN1 (FULL_SIMP_TAC (srw_ss()) [f_o_f_DEF,SUBSET_DEF])
-  THEN1
-   (FULL_SIMP_TAC std_ss [ONCE_REWRITE_RULE [CONJ_COMM] EVERY2_EVERY,
-      LENGTH_ADDR_MAP,EVERY_MEM,MEM_ZIP,PULL_EXISTS] \\ REPEAT STRIP_TAC \\ RES_TAC
-    \\ FULL_SIMP_TAC std_ss [MEM_ZIP,PULL_EXISTS]
-    \\ `MEM (EL n roots) roots` by (FULL_SIMP_TAC std_ss [MEM_EL] \\ METIS_TAC [])
-    \\ `(!ptr. (EL n roots = Pointer ptr) ==> ptr IN FDOM g)` by METIS_TAC []
-    \\ IMP_RES_TAC bc_value_inv_related \\ IMP_RES_TAC EL_ADDR_MAP
-    \\ FULL_SIMP_TAC std_ss [])
-  \\ MATCH_MP_TAC bc_ref_inv_related \\ FULL_SIMP_TAC std_ss []
-  \\ METIS_TAC [reachable_refs_lemma]);
-
-val full_gc_thm = store_thm("full_gc_thm",
-  ``abs_ml_inv stack refs (roots,heap,a,sp) limit ==>
-    ?roots2 heap2 a2.
-      (full_gc (roots,heap,limit) = (roots2,heap2,a2,T)) /\
-      abs_ml_inv stack refs
-        (roots2,heap2 ++ heap_expand (limit - a2),a2,limit - a2) limit /\
-      (heap_length heap2 = a2)``,
-  SIMP_TAC std_ss [abs_ml_inv_def,GSYM CONJ_ASSOC]
-  \\ REPEAT STRIP_TAC \\ IMP_RES_TAC full_gc_related \\ NTAC 3 (POP_ASSUM (K ALL_TAC))
-  \\ `heap_length heap2 = a2` by ALL_TAC
-  THEN1 (IMP_RES_TAC full_gc_LENGTH \\ FULL_SIMP_TAC std_ss [] \\ METIS_TAC [])
-  \\ `unused_space_inv a2 (limit - a2) (heap2 ++ heap_expand (limit - a2))` by
-   (FULL_SIMP_TAC std_ss [unused_space_inv_def] \\ REPEAT STRIP_TAC
-    \\ FULL_SIMP_TAC std_ss [heap_expand_def]
-    \\ METIS_TAC [heap_lookup_PREFIX])
-  \\ FULL_SIMP_TAC std_ss [] \\ SIMP_TAC std_ss [CONJ_ASSOC] \\ STRIP_TAC THEN1
-   (Q.PAT_ASSUM `full_gc (roots,heap,limit) = xxx` (ASSUME_TAC o GSYM)
-    \\ IMP_RES_TAC full_gc_ok \\ NTAC 3 (POP_ASSUM (K ALL_TAC))
-    \\ FULL_SIMP_TAC std_ss [] \\ METIS_TAC [])
-  \\ MATCH_MP_TAC (GEN_ALL bc_stack_ref_inv_related) \\ FULL_SIMP_TAC std_ss []
-  \\ Q.EXISTS_TAC `heap` \\ FULL_SIMP_TAC std_ss []);
-
-(* Write to unused heap space is fine, e.g. cons *)
-
-val heap_store_def = Define `
-  (heap_store a y [] = ([],F)) /\
-  (heap_store a y (x::xs) =
-    if a = 0 then (y ++ xs, el_length x = heap_length y) else
-    if a < el_length x then (x::xs,F) else
-      let (xs,c) = heap_store (a - el_length x) y xs in
-        (x::xs,c))`
-
-val isUnused_def = Define `
-  isUnused x = ?k. x = Unused k`;
-
-val isSomeUnused_def = Define `
-  isSomeUnused x = ?k. x = SOME (Unused k)`;
-
-val heap_store_unused_def = Define `
-  heap_store_unused a sp x xs =
-    if (heap_lookup a xs = SOME (Unused (sp-1))) /\ el_length x <= sp then
-      heap_store a (heap_expand (sp - el_length x) ++ [x]) xs
-    else (xs,F)`;
-
-val heap_store_lemma = store_thm("heap_store_lemma",
-  ``!xs y x ys.
-      heap_store (heap_length xs) y (xs ++ x::ys) =
-      (xs ++ y ++ ys, heap_length y = el_length x)``,
-  Induct \\ FULL_SIMP_TAC (srw_ss()) [heap_length_def,heap_store_def,LET_DEF]
-  THEN1 DECIDE_TAC \\ REPEAT STRIP_TAC
-  \\ `el_length h <> 0` by (Cases_on `h` \\ FULL_SIMP_TAC std_ss [el_length_def])
-  \\ `~(el_length h + SUM (MAP el_length xs) < el_length h)` by DECIDE_TAC
-  \\ FULL_SIMP_TAC std_ss []);
-
-val heap_store_rel_def = Define `
-  heap_store_rel heap heap2 =
-    (!ptr. isSomeDataElement (heap_lookup ptr heap) ==>
-           (heap_lookup ptr heap2 = heap_lookup ptr heap))`;
-
-val isSomeDataElement_heap_lookup_lemma1 = prove(
-  ``isSomeDataElement (heap_lookup n (Unused k :: xs)) =
-    k < n /\ isSomeDataElement (heap_lookup (n-(k+1)) xs)``,
-  SRW_TAC [] [heap_lookup_def,isSomeDataElement_def,el_length_def,NOT_LESS]
-  THEN1 (DISJ1_TAC \\ DECIDE_TAC)
-  \\ `k < n` by DECIDE_TAC \\ FULL_SIMP_TAC std_ss []);
-
-val isSomeDataElement_heap_lookup_lemma2 = prove(
-  ``isSomeDataElement (heap_lookup n (heap_expand k ++ xs)) =
-    k <= n /\ isSomeDataElement (heap_lookup (n-k) xs)``,
-  SRW_TAC [] [heap_expand_def,isSomeDataElement_heap_lookup_lemma1]
-  \\ IMP_RES_TAC (DECIDE ``sp <> 0 ==> (sp - 1 + 1 = sp:num)``)
-  \\ FULL_SIMP_TAC std_ss []
-  \\ Cases_on `isSomeDataElement (heap_lookup (n - k) xs)`
-  \\ FULL_SIMP_TAC std_ss [] \\ DECIDE_TAC);
-
-val isSomeDataElement_heap_lookup_lemma3 = prove(
-  ``n <> 0 ==>
-    (isSomeDataElement (heap_lookup n (x::xs)) =
-     el_length x <= n /\ isSomeDataElement (heap_lookup (n - el_length x) xs))``,
-  SRW_TAC [] [heap_expand_def,heap_lookup_def,isSomeDataElement_def]
-  THEN1 (DISJ1_TAC \\ DECIDE_TAC)
-  \\ `el_length x <= n` by DECIDE_TAC \\ FULL_SIMP_TAC std_ss []);
-
-val IMP_heap_store_unused = prove(
-  ``unused_space_inv a sp (heap:('a,'b) heap_element list) /\ el_length x <= sp ==>
-    ?heap2. (heap_store_unused a sp x heap = (heap2,T)) /\
-            unused_space_inv a (sp - el_length x) heap2 /\
-            (heap_lookup (a + sp - el_length x) heap2 = SOME x) /\
-            ~isSomeDataElement (heap_lookup (a + sp - el_length x) heap) /\
-            (heap_length heap2 = heap_length heap) /\
-            (~isForwardPointer x ==>
-             (FILTER isForwardPointer heap2 = FILTER isForwardPointer heap)) /\
-            (!xs l d.
-               MEM (DataElement xs l d) heap2 = (x = DataElement xs l d) \/
-                                                MEM (DataElement xs l d) heap) /\
-            (isDataElement x ==>
-             ({a | isSomeDataElement (heap_lookup a heap2)} =
-               a + sp - el_length x INSERT {a | isSomeDataElement (heap_lookup a heap)})) /\
-            heap_store_rel heap heap2``,
-  REPEAT STRIP_TAC \\ ASM_SIMP_TAC std_ss [heap_store_unused_def,heap_store_rel_def]
-  \\ `sp <> 0` by (Cases_on `x` \\ FULL_SIMP_TAC std_ss [el_length_def] \\ DECIDE_TAC)
-  \\ FULL_SIMP_TAC std_ss [unused_space_inv_def]
-  \\ IMP_RES_TAC heap_lookup_SPLIT \\ FULL_SIMP_TAC std_ss []
-  \\ FULL_SIMP_TAC std_ss [heap_store_lemma]
-  \\ STRIP_TAC THEN1
-   (FULL_SIMP_TAC (srw_ss()) [heap_length_def,SUM_APPEND,el_length_def]
-    \\ FULL_SIMP_TAC std_ss [GSYM heap_length_def,heap_length_heap_expand]
-    \\ DECIDE_TAC)
-  \\ STRIP_TAC THEN1
-   (REPEAT STRIP_TAC \\ FULL_SIMP_TAC std_ss
-      [heap_expand_def,APPEND,GSYM APPEND_ASSOC,heap_lookup_PREFIX])
-  \\ STRIP_TAC THEN1
-   (FULL_SIMP_TAC std_ss [GSYM APPEND_ASSOC,APPEND]
-    \\ FULL_SIMP_TAC std_ss [APPEND_ASSOC]
-    \\ `heap_length ha + sp - el_length x =
-        heap_length (ha ++ heap_expand (sp - el_length x))` by
-     (FULL_SIMP_TAC std_ss [heap_length_APPEND,heap_length_heap_expand] \\ DECIDE_TAC)
-    \\ FULL_SIMP_TAC std_ss [heap_lookup_PREFIX])
-  \\ STRIP_TAC THEN1
-   (`~(heap_length ha + sp - el_length x < heap_length ha)` by DECIDE_TAC
-    \\ IMP_RES_TAC NOT_LESS_IMP_heap_lookup
-    \\ FULL_SIMP_TAC std_ss []
-    \\ `heap_length ha + sp - el_length x - heap_length ha =
-        sp - el_length x` by DECIDE_TAC \\ FULL_SIMP_TAC std_ss []
-    \\ SIMP_TAC std_ss [heap_lookup_def]
-    \\ SRW_TAC [] [isSomeDataElement_def,el_length_def]
-    \\ REVERSE (FULL_SIMP_TAC std_ss []) THEN1 (`F` by DECIDE_TAC)
-    \\ Cases_on `x` \\ FULL_SIMP_TAC std_ss [el_length_def]
-    \\ `F` by DECIDE_TAC)
-  \\ STRIP_TAC THEN1
-   (FULL_SIMP_TAC (srw_ss()) [heap_length_APPEND,heap_length_heap_expand,
-      heap_length_def,el_length_def] \\ DECIDE_TAC)
-  \\ STRIP_TAC THEN1
-   (FULL_SIMP_TAC std_ss [FILTER_APPEND,FILTER,isForwardPointer_def,APPEND_NIL]
-    \\ SRW_TAC [] [heap_expand_def,isForwardPointer_def])
-  \\ STRIP_TAC THEN1
-   (FULL_SIMP_TAC (srw_ss()) [MEM_APPEND,MEM,heap_expand_def]
-    \\ Cases_on `sp <= el_length x` \\ FULL_SIMP_TAC (srw_ss()) []
-    \\ METIS_TAC [])
-  \\ STRIP_TAC THEN1
-   (REPEAT STRIP_TAC \\ FULL_SIMP_TAC (srw_ss()) [EXTENSION]
-    \\ STRIP_TAC \\ Q.ABBREV_TAC `y = x'` \\ POP_ASSUM (K ALL_TAC)
-    \\ Cases_on `y = heap_length ha + sp - el_length x`
-    \\ FULL_SIMP_TAC std_ss [] THEN1
-     (ONCE_REWRITE_TAC [GSYM APPEND_ASSOC] \\ SIMP_TAC std_ss [APPEND]
-      \\ `(heap_length ha + sp - el_length x) =
-          heap_length (ha ++ heap_expand (sp - el_length x))` by
-       (FULL_SIMP_TAC std_ss [heap_length_APPEND,heap_length_heap_expand]
-        \\ DECIDE_TAC)
-      \\ FULL_SIMP_TAC std_ss [heap_lookup_PREFIX]
-      \\ FULL_SIMP_TAC (srw_ss()) [isDataElement_def,isSomeDataElement_def])
-    \\ Cases_on `y < heap_length ha`
-    THEN1 (FULL_SIMP_TAC std_ss [LESS_IMP_heap_lookup,GSYM APPEND_ASSOC])
-    \\ IMP_RES_TAC NOT_LESS_IMP_heap_lookup
-    \\ FULL_SIMP_TAC std_ss [GSYM APPEND_ASSOC]
-    \\ FULL_SIMP_TAC std_ss [isSomeDataElement_heap_lookup_lemma1,
-         isSomeDataElement_heap_lookup_lemma2]
-    \\ `0 < el_length x` by
-         (Cases_on `x` \\ FULL_SIMP_TAC std_ss [el_length_def] \\ DECIDE_TAC)
-    \\ REVERSE (Cases_on `sp <= el_length x + (y - heap_length ha)`)
-    \\ FULL_SIMP_TAC std_ss []
-    THEN1 (CCONTR_TAC \\ FULL_SIMP_TAC std_ss [] \\ DECIDE_TAC)
-    \\ `0 < y - heap_length ha` by DECIDE_TAC
-    \\ FULL_SIMP_TAC std_ss []
-    \\ `y - heap_length ha - (sp - el_length x) <> 0` by DECIDE_TAC
-    \\ FULL_SIMP_TAC std_ss [APPEND,isSomeDataElement_heap_lookup_lemma3]
-    \\ REVERSE (Cases_on `el_length x <= y - heap_length ha - (sp - el_length x)`)
-    \\ FULL_SIMP_TAC std_ss []
-    THEN1 (CCONTR_TAC \\ FULL_SIMP_TAC std_ss [] \\ DECIDE_TAC)
-    \\ `sp < 1 + (y - heap_length ha)` by DECIDE_TAC
-    \\ FULL_SIMP_TAC std_ss [SUB_SUB]
-    \\ IMP_RES_TAC (DECIDE ``sp <> 0 ==> (sp - 1 + 1 = sp:num)``)
-    \\ FULL_SIMP_TAC std_ss []
-    \\ IMP_RES_TAC (DECIDE  ``n <= sp ==> (y - m + n - sp - n = y - m - sp:num)``)
-    \\ FULL_SIMP_TAC std_ss [])
-  \\ REPEAT STRIP_TAC
-  \\ FULL_SIMP_TAC std_ss [isSomeDataElement_def]
-  \\ Cases_on `ptr < heap_length ha`
-  THEN1 (IMP_RES_TAC LESS_IMP_heap_lookup \\ FULL_SIMP_TAC std_ss [GSYM APPEND_ASSOC])
-  \\ IMP_RES_TAC NOT_LESS_IMP_heap_lookup \\ FULL_SIMP_TAC std_ss [GSYM APPEND_ASSOC]
-  \\ POP_ASSUM (K ALL_TAC) \\ Q.PAT_ASSUM `xxx = SOME yyy` MP_TAC
-  \\ SIMP_TAC std_ss [Once heap_lookup_def] \\ SRW_TAC [] []
-  \\ `~(ptr - heap_length ha < heap_length (heap_expand (sp - el_length x) ++ [x]))` by
-   (FULL_SIMP_TAC (srw_ss()) [heap_length_APPEND,heap_length_heap_expand,
-      el_length_def,heap_length_def] \\ DECIDE_TAC)
-  \\ IMP_RES_TAC NOT_LESS_IMP_heap_lookup \\ POP_ASSUM (K ALL_TAC)
-  \\ POP_ASSUM (fn th => ONCE_REWRITE_TAC [th])
-  \\ `heap_length (heap_expand (sp - el_length x) ++ [x]) = sp` by
-   (FULL_SIMP_TAC (srw_ss()) [heap_length_APPEND,heap_length_heap_expand,
-      el_length_def,heap_length_def] \\ DECIDE_TAC)
-  \\ `el_length (Unused (sp - 1)) = sp` by
-   (FULL_SIMP_TAC (srw_ss()) [heap_length_APPEND,heap_length_heap_expand,
-      el_length_def,heap_length_def] \\ DECIDE_TAC)
-  \\ FULL_SIMP_TAC std_ss []);
-
-val heap_store_rel_lemma = prove(
-  ``heap_store_rel h1 h2 /\ (heap_lookup n h1 = SOME (DataElement ys l d)) ==>
-    (heap_lookup n h2 = SOME (DataElement ys l d))``,
-  SIMP_TAC std_ss [heap_store_rel_def,isSomeDataElement_def] \\ METIS_TAC []);
 
 (* Lemmas about ok and a *)
 
@@ -1357,605 +909,5 @@ val th = MP th lemma |> SIMP_RULE std_ss []
          |> Q.SPECL [`h1`,`h2`,`a`,`n`,`heap`,`c`,`limit`,`h1'`,`a'`,`n'`,`heap'`]
 
 val gc_move_loop_ok = save_thm("gc_move_loop_ok",th);
-
-(* cons *)
-
-val EVERY2_APPEND_IMP = prove(
-  ``!xs1 xs2 ys.
-      EVERY2 P (xs1 ++ xs2) ys ==>
-      ?ys1 ys2. (ys = ys1 ++ ys2) /\ EVERY2 P xs1 ys1 /\ EVERY2 P xs2 ys2``,
-  Induct \\ FULL_SIMP_TAC (srw_ss()) []
-  \\ Cases_on `ys` \\ FULL_SIMP_TAC (srw_ss()) [] \\ REPEAT STRIP_TAC
-  \\ RES_TAC \\ METIS_TAC [EVERY2_def,APPEND]);
-
-val INJ_SUBSET = prove(
-  ``!x y z. INJ f x y /\ y SUBSET z ==> INJ f x z``,
-  FULL_SIMP_TAC (srw_ss()) [INJ_DEF,SUBSET_DEF]);
-
-val bc_value_inv_SUBMAP = prove(
-  ``!w x.
-      f SUBMAP f1 /\ heap_store_rel heap heap1 /\
-      bc_value_inv w (x,f,heap) ==>
-      bc_value_inv w (x,f1,heap1) ``,
-  completeInduct_on `bc_value_size w` \\ NTAC 3 STRIP_TAC
-  \\ FULL_SIMP_TAC std_ss [PULL_FORALL] \\ Cases_on `w` THEN1
-   (FULL_SIMP_TAC std_ss [bc_value_inv_def,DataOnly_def] \\ SRW_TAC [] []
-    \\ IMP_RES_TAC heap_store_rel_lemma \\ FULL_SIMP_TAC std_ss [])
-  THEN1 (FULL_SIMP_TAC (srw_ss()) [bc_value_inv_def,ADDR_APPLY_def,BlockRep_def]
-    \\ Cases_on `l = []` \\ FULL_SIMP_TAC std_ss []
-    \\ FULL_SIMP_TAC (srw_ss()) [bc_value_inv_def,ADDR_APPLY_def,BlockRep_def]
-    \\ REPEAT STRIP_TAC
-    \\ FULL_SIMP_TAC std_ss [EVERY2_EVERY,LENGTH_ADDR_MAP,EVERY_MEM,FORALL_PROD]
-    \\ Q.PAT_ASSUM `LENGTH l = LENGTH xs` ASSUME_TAC
-    \\ FULL_SIMP_TAC (srw_ss()) [MEM_ZIP,LENGTH_ADDR_MAP,PULL_EXISTS]
-    \\ IMP_RES_TAC heap_store_rel_lemma \\ FULL_SIMP_TAC (srw_ss()) []
-    \\ FULL_SIMP_TAC (srw_ss()) [MEM_ZIP,LENGTH_ADDR_MAP,PULL_EXISTS]
-    \\ REPEAT STRIP_TAC
-    \\ Q.MATCH_ASSUM_RENAME_TAC `t < LENGTH xs` [] \\ RES_TAC
-    \\ `MEM (EL t l) l` by (FULL_SIMP_TAC std_ss [MEM_EL] \\ METIS_TAC [])
-    \\ `bc_value_size (EL t l) < bc_value_size (Block n l)` by ALL_TAC THEN1
-     (FULL_SIMP_TAC std_ss [bc_value_size_def]
-      \\ IMP_RES_TAC MEM_IMP_bc_value_size \\ DECIDE_TAC) \\ RES_TAC)
-  THEN1 (FULL_SIMP_TAC std_ss [bc_value_inv_def])
-  THEN1 (FULL_SIMP_TAC (srw_ss()) [bc_value_inv_def,SUBMAP_DEF])
-  THEN1 (FULL_SIMP_TAC std_ss [bc_value_inv_def]));
-
-val EVERY2_LENGTH = prove(
-  ``!xs ys. EVERY2 P xs ys ==> (LENGTH xs = LENGTH ys)``,
-  Induct \\ Cases_on `ys` \\ FULL_SIMP_TAC (srw_ss()) []);
-
-val cons_thm = store_thm("cons_thm",
-  ``abs_ml_inv (xs ++ stack) refs (roots,heap,a,sp) limit /\
-    LENGTH xs < sp /\ xs <> [] ==>
-    ?rs roots2 heap2.
-      (roots = rs ++ roots2) /\ (LENGTH rs = LENGTH xs) /\
-      (heap_store_unused a sp (BlockRep tag rs) heap = (heap2,T)) /\
-      abs_ml_inv ((Block tag xs)::stack) refs
-                 (Pointer (a + sp - el_length (BlockRep tag rs))::roots2,heap2,a,
-                  sp-el_length (BlockRep tag rs)) limit``,
-  SIMP_TAC std_ss [abs_ml_inv_def]
-  \\ REPEAT STRIP_TAC \\ FULL_SIMP_TAC std_ss [bc_stack_ref_inv_def,EVERY2_def]
-  \\ IMP_RES_TAC EVERY2_APPEND_IMP \\ FULL_SIMP_TAC std_ss []
-  \\ Q.LIST_EXISTS_TAC [`ys1`,`ys2`] \\ FULL_SIMP_TAC std_ss []
-  \\ IMP_RES_TAC EVERY2_LENGTH \\ FULL_SIMP_TAC std_ss []
-  \\ Q.PAT_ASSUM `unused_space_inv a sp heap` (fn th =>
-    MATCH_MP (IMP_heap_store_unused |> REWRITE_RULE [GSYM AND_IMP_INTRO] |> GEN_ALL) th
-    |> ASSUME_TAC)
-  \\ POP_ASSUM (MP_TAC o Q.SPEC `(BlockRep tag ys1)`) \\ MATCH_MP_TAC IMP_IMP
-  \\ STRIP_TAC THEN1 (FULL_SIMP_TAC std_ss [BlockRep_def,el_length_def] \\ DECIDE_TAC)
-  \\ STRIP_TAC \\ FULL_SIMP_TAC std_ss []
-  \\ STRIP_TAC THEN1
-   (FULL_SIMP_TAC (srw_ss()) [roots_ok_def,MEM,BlockRep_def]
-    \\ REVERSE (REPEAT STRIP_TAC \\ RES_TAC) THEN1 METIS_TAC [heap_store_rel_def]
-    \\ FULL_SIMP_TAC (srw_ss()) [el_length_def,isSomeDataElement_def])
-  \\ STRIP_TAC THEN1
-   (FULL_SIMP_TAC (srw_ss()) [roots_ok_def,MEM,BlockRep_def,heap_ok_def,
-      isForwardPointer_def] \\ ONCE_REWRITE_TAC [EQ_SYM_EQ]
-    \\ REPEAT STRIP_TAC \\ METIS_TAC [heap_store_rel_def])
-  \\ STRIP_TAC THEN1 (FULL_SIMP_TAC std_ss [el_length_def,BlockRep_def])
-  \\ Q.EXISTS_TAC `f` \\ FULL_SIMP_TAC std_ss []
-  \\ STRIP_TAC THEN1
-   (MATCH_MP_TAC INJ_SUBSET
-    \\ Q.EXISTS_TAC `{a | isSomeDataElement (heap_lookup a heap)}`
-    \\ FULL_SIMP_TAC (srw_ss()) [isDataElement_def,BlockRep_def])
-  \\ REPEAT STRIP_TAC THEN1
-   (FULL_SIMP_TAC (srw_ss()) [bc_value_inv_def]
-    \\ FULL_SIMP_TAC std_ss [BlockRep_def,el_length_def]
-    \\ Q.EXISTS_TAC `ys1` \\ FULL_SIMP_TAC std_ss []
-    \\ FULL_SIMP_TAC std_ss [EVERY2_EVERY,EVERY_MEM,MEM_ZIP,PULL_EXISTS]
-    \\ `f SUBMAP f` by FULL_SIMP_TAC std_ss [SUBMAP_REFL]
-    \\ REPEAT STRIP_TAC \\ RES_TAC \\ IMP_RES_TAC bc_value_inv_SUBMAP)
-  THEN1
-   (FULL_SIMP_TAC std_ss [EVERY2_EVERY,EVERY_MEM,MEM_ZIP,PULL_EXISTS]
-    \\ `f SUBMAP f` by FULL_SIMP_TAC std_ss [SUBMAP_REFL]
-    \\ REPEAT STRIP_TAC \\ RES_TAC \\ IMP_RES_TAC bc_value_inv_SUBMAP)
-  \\ `reachable_refs (xs++stack) refs n` by ALL_TAC THEN1
-   (POP_ASSUM MP_TAC \\ SIMP_TAC std_ss [reachable_refs_def]
-    \\ REPEAT STRIP_TAC \\ FULL_SIMP_TAC std_ss [MEM] THEN1
-     (NTAC 2 (POP_ASSUM MP_TAC) \\ FULL_SIMP_TAC std_ss []
-      \\ FULL_SIMP_TAC std_ss [get_refs_def,MEM_FLAT,MEM_MAP,PULL_EXISTS]
-      \\ FULL_SIMP_TAC std_ss [MEM_APPEND] \\ METIS_TAC [])
-    \\ FULL_SIMP_TAC std_ss [MEM_APPEND] \\ METIS_TAC [])
-  \\ RES_TAC \\ POP_ASSUM MP_TAC \\ SIMP_TAC std_ss [bc_ref_inv_def]
-  \\ REPEAT STRIP_TAC \\ FULL_SIMP_TAC std_ss [RefBlock_def]
-  \\ IMP_RES_TAC heap_store_rel_lemma \\ FULL_SIMP_TAC (srw_ss()) []
-  \\ `f SUBMAP f` by FULL_SIMP_TAC std_ss [SUBMAP_REFL]
-  \\ REPEAT STRIP_TAC \\ RES_TAC \\ IMP_RES_TAC bc_value_inv_SUBMAP)
-
-val cons_thm_EMPTY = store_thm("cons_thm_EMPTY",
-  ``abs_ml_inv stack refs (roots,heap:('a,'b) ml_heap,a,sp) limit /\
-    tag < 2 ** 62 ==>
-    abs_ml_inv ((Block tag [])::stack) refs
-                (Data (2w * n2w tag + 1w)::roots,heap,a,sp) limit``,
-  SIMP_TAC std_ss [abs_ml_inv_def] \\ REPEAT STRIP_TAC
-  \\ FULL_SIMP_TAC std_ss [bc_stack_ref_inv_def,EVERY2_def]
-  \\ FULL_SIMP_TAC (srw_ss()) [roots_ok_def,MEM]
-  \\ Q.EXISTS_TAC `f` \\ FULL_SIMP_TAC std_ss []
-  \\ FULL_SIMP_TAC (srw_ss()) [bc_value_inv_def]
-  \\ REPEAT STRIP_TAC \\ `reachable_refs stack refs n` by ALL_TAC \\ RES_TAC
-  \\ FULL_SIMP_TAC std_ss [reachable_refs_def]
-  \\ Cases_on `x = Block tag []` \\ FULL_SIMP_TAC std_ss []
-  \\ FULL_SIMP_TAC (srw_ss()) [get_refs_def] \\ METIS_TAC []);
-
-(* update ref *)
-
-val reachable_refs_UPDATE = prove(
-  ``reachable_refs (x::RefPtr ptr::stack) (refs |+ (ptr,x)) n ==>
-    reachable_refs (x::RefPtr ptr::stack) refs n``,
-  FULL_SIMP_TAC std_ss [reachable_refs_def] \\ REPEAT STRIP_TAC
-  \\ Cases_on `?m. MEM m (get_refs x) /\ RTC (ref_edge refs) m n` THEN1
-   (FULL_SIMP_TAC std_ss [] \\ Q.LIST_EXISTS_TAC [`x`,`m`]
-    \\ FULL_SIMP_TAC std_ss [MEM])
-  \\ FULL_SIMP_TAC std_ss [] \\ Q.LIST_EXISTS_TAC [`x'`,`r`]
-  \\ FULL_SIMP_TAC std_ss [METIS_PROVE [] ``~b \/ c = b ==> c``]
-  \\ FULL_SIMP_TAC std_ss [RTC_eq_NRC]
-  \\ Q.ABBREV_TAC `k = n'` \\ POP_ASSUM (K ALL_TAC) \\ Q.EXISTS_TAC `k`
-  \\ POP_ASSUM MP_TAC \\ POP_ASSUM MP_TAC \\ REPEAT (POP_ASSUM (K ALL_TAC))
-  \\ Q.SPEC_TAC (`r`,`r`) \\ Induct_on `k`
-  \\ FULL_SIMP_TAC std_ss [NRC]
-  \\ REPEAT STRIP_TAC \\ FULL_SIMP_TAC std_ss [] \\ RES_TAC
-  \\ Q.EXISTS_TAC `z` \\ FULL_SIMP_TAC std_ss []
-  \\ FULL_SIMP_TAC std_ss [ref_edge_def]
-  \\ REVERSE (Cases_on `r = ptr`)
-  \\ FULL_SIMP_TAC (srw_ss()) [FDOM_FUPDATE,FAPPLY_FUPDATE_THM]
-  \\ METIS_TAC []);
-
-val isRefBlock_def = Define `
-  isRefBlock x = ?p. x = RefBlock p`;
-
-val RefBlock_inv_def = Define `
-  RefBlock_inv heap heap2 =
-    (!n x. (heap_lookup n heap = SOME x) /\ ~(isRefBlock x) ==>
-           (heap_lookup n heap2 = SOME x)) /\
-    (!n x. (heap_lookup n heap2 = SOME x) /\ ~(isRefBlock x) ==>
-           (heap_lookup n heap = SOME x))`;
-
-val heap_store_RefBlock_thm = prove(
-  ``!ha. heap_store (heap_length ha) [RefBlock x] (ha ++ RefBlock y::hb) =
-           (ha ++ RefBlock x::hb,T)``,
-  Induct \\ FULL_SIMP_TAC (srw_ss()) [heap_store_def,heap_length_def]
-  THEN1 FULL_SIMP_TAC std_ss [RefBlock_def,el_length_def] \\ STRIP_TAC
-  \\ `~(el_length h + SUM (MAP el_length ha) < el_length h) /\ el_length h <> 0` by
-       (Cases_on `h` \\ FULL_SIMP_TAC std_ss [el_length_def] \\ DECIDE_TAC)
-  \\ FULL_SIMP_TAC std_ss [LET_DEF]);
-
-val heap_lookup_RefBlock_lemma = prove(
-  ``(heap_lookup n (ha ++ RefBlock y::hb) = SOME x) =
-      if n < heap_length ha then
-        (heap_lookup n ha = SOME x)
-      else if n = heap_length ha then
-        (x = RefBlock y)
-      else if heap_length ha + 2 <= n then
-        (heap_lookup (n - heap_length ha - 2) hb = SOME x)
-      else F``,
-  Cases_on `n < heap_length ha` \\ FULL_SIMP_TAC std_ss [LESS_IMP_heap_lookup]
-  \\ FULL_SIMP_TAC std_ss [NOT_LESS_IMP_heap_lookup]
-  \\ FULL_SIMP_TAC std_ss [heap_lookup_def]
-  \\ Cases_on `n <= heap_length ha` \\ FULL_SIMP_TAC std_ss []
-  THEN1 (`heap_length ha = n` by DECIDE_TAC \\ FULL_SIMP_TAC std_ss [] \\ METIS_TAC [])
-  \\ `heap_length ha <> n` by DECIDE_TAC \\ FULL_SIMP_TAC std_ss []
-  \\ `0 < el_length (RefBlock y)` by FULL_SIMP_TAC std_ss [el_length_def,RefBlock_def]
-  \\ FULL_SIMP_TAC std_ss [] \\ SRW_TAC [] []
-  \\ FULL_SIMP_TAC std_ss [el_length_def,RefBlock_def,NOT_LESS]
-  \\ DISJ1_TAC \\ DECIDE_TAC);
-
-val heap_store_RefBlock = prove(
-  ``(heap_lookup n heap = SOME (RefBlock y)) ==>
-    ?heap2. (heap_store n [RefBlock h] heap = (heap2,T)) /\
-            RefBlock_inv heap heap2 /\
-            (heap_lookup n heap2 = SOME (RefBlock h)) /\
-            (heap_length heap2 = heap_length heap) /\
-            (FILTER isForwardPointer heap2 = FILTER isForwardPointer heap) /\
-            (!xs l d.
-               MEM (DataElement xs l d) heap2 ==> (DataElement xs l d = RefBlock h) \/
-                                                  MEM (DataElement xs l d) heap) /\
-            (!a. isSomeDataElement (heap_lookup a heap2) =
-                 isSomeDataElement (heap_lookup a heap)) /\
-            !m x. m <> n /\ (heap_lookup m heap = SOME x) ==>
-                  (heap_lookup m heap2 = SOME x)``,
-  REPEAT STRIP_TAC \\ IMP_RES_TAC heap_lookup_SPLIT
-  \\ FULL_SIMP_TAC std_ss [heap_store_RefBlock_thm]
-  \\ STRIP_TAC THEN1
-   (FULL_SIMP_TAC std_ss [RefBlock_inv_def]
-    \\ FULL_SIMP_TAC std_ss [heap_lookup_RefBlock_lemma]
-    \\ FULL_SIMP_TAC std_ss [isRefBlock_def] \\ METIS_TAC [])
-  \\ STRIP_TAC THEN1 (FULL_SIMP_TAC std_ss [heap_lookup_PREFIX])
-  \\ STRIP_TAC THEN1 (FULL_SIMP_TAC (srw_ss())
-       [heap_length_APPEND,heap_length_def,RefBlock_def,el_length_def])
-  \\ STRIP_TAC THEN1
-   (FULL_SIMP_TAC (srw_ss()) [FILTER_APPEND,FILTER,isForwardPointer_def,RefBlock_def])
-  \\ STRIP_TAC THEN1
-   (FULL_SIMP_TAC (srw_ss()) [MEM,MEM_APPEND,RefBlock_def] \\ METIS_TAC [])
-  \\ STRIP_TAC THEN1
-   (FULL_SIMP_TAC std_ss [isSomeDataElement_def,heap_lookup_RefBlock_lemma]
-    \\ FULL_SIMP_TAC std_ss [RefBlock_def] \\ METIS_TAC [])
-  \\ FULL_SIMP_TAC std_ss [isSomeDataElement_def,heap_lookup_RefBlock_lemma]
-  \\ METIS_TAC []);
-
-val NOT_isRefBlock = prove(
-  ``~(isRefBlock (DataOnly x y)) /\
-    ~(isRefBlock (DataElement xs (LENGTH xs) (BlockTag n,[])))``,
-  SIMP_TAC (srw_ss()) [isRefBlock_def,DataOnly_def,RefBlock_def]);
-
-val bc_value_inv_Ref = prove(
-  ``RefBlock_inv heap heap2 ==>
-    !x h f. (bc_value_inv x (h,f,heap2) = bc_value_inv x (h,f,heap))``,
-  STRIP_TAC \\ completeInduct_on `bc_value_size x` \\ NTAC 3 STRIP_TAC
-  \\ FULL_SIMP_TAC std_ss [PULL_FORALL] \\ Cases_on `x` THEN1
-   (FULL_SIMP_TAC std_ss [bc_value_inv_def] \\ SRW_TAC [] []
-    \\ REPEAT STRIP_TAC \\ FULL_SIMP_TAC std_ss []
-    \\ FULL_SIMP_TAC std_ss [RefBlock_inv_def]
-    \\ METIS_TAC [NOT_isRefBlock])
-  THEN1 (FULL_SIMP_TAC (srw_ss()) [bc_value_inv_def,ADDR_APPLY_def,BlockRep_def]
-    \\ Cases_on `l = []` \\ FULL_SIMP_TAC std_ss []
-    \\ FULL_SIMP_TAC (srw_ss()) [bc_value_inv_def,ADDR_APPLY_def,BlockRep_def]
-    \\ REPEAT STRIP_TAC
-    \\ FULL_SIMP_TAC std_ss [EVERY2_EVERY,LENGTH_ADDR_MAP,EVERY_MEM,FORALL_PROD]
-    \\ REPEAT STRIP_TAC \\ EQ_TAC \\ REPEAT STRIP_TAC
-    THEN1
-     (Q.PAT_ASSUM `LENGTH l = LENGTH xs` ASSUME_TAC
-      \\ FULL_SIMP_TAC (srw_ss()) [MEM_ZIP,LENGTH_ADDR_MAP,PULL_EXISTS]
-      \\ `heap_lookup ptr heap =
-           SOME (DataElement xs (LENGTH xs) (BlockTag n,[]))` by
-              METIS_TAC [RefBlock_inv_def,NOT_isRefBlock]
-      \\ FULL_SIMP_TAC (srw_ss()) [MEM_ZIP]
-      \\ REPEAT STRIP_TAC
-      \\ Q.MATCH_ASSUM_RENAME_TAC `t < LENGTH xs` [] \\ RES_TAC
-      \\ `MEM (EL t l) l` by (FULL_SIMP_TAC std_ss [MEM_EL] \\ METIS_TAC [])
-      \\ `bc_value_size (EL t l) < bc_value_size (Block n l)` by ALL_TAC THEN1
-       (FULL_SIMP_TAC std_ss [bc_value_size_def]
-        \\ IMP_RES_TAC MEM_IMP_bc_value_size \\ DECIDE_TAC) \\ RES_TAC
-      \\ FULL_SIMP_TAC std_ss [])
-    THEN1
-     (Q.PAT_ASSUM `LENGTH l = LENGTH xs` ASSUME_TAC
-      \\ FULL_SIMP_TAC (srw_ss()) [MEM_ZIP,LENGTH_ADDR_MAP,PULL_EXISTS]
-      \\ `heap_lookup ptr heap2 =
-           SOME (DataElement xs (LENGTH xs) (BlockTag n,[]))` by
-              METIS_TAC [RefBlock_inv_def,NOT_isRefBlock]
-      \\ FULL_SIMP_TAC (srw_ss()) [MEM_ZIP]
-      \\ REPEAT STRIP_TAC
-      \\ Q.MATCH_ASSUM_RENAME_TAC `t < LENGTH xs` [] \\ RES_TAC
-      \\ `MEM (EL t l) l` by (FULL_SIMP_TAC std_ss [MEM_EL] \\ METIS_TAC [])
-      \\ `bc_value_size (EL t l) < bc_value_size (Block n l)` by ALL_TAC THEN1
-       (FULL_SIMP_TAC std_ss [bc_value_size_def]
-        \\ IMP_RES_TAC MEM_IMP_bc_value_size \\ DECIDE_TAC) \\ RES_TAC
-      \\ FULL_SIMP_TAC std_ss []))
-  THEN1 (FULL_SIMP_TAC std_ss [bc_value_inv_def])
-  THEN1 (FULL_SIMP_TAC (srw_ss()) [bc_value_inv_def,SUBMAP_DEF])
-  THEN1 (FULL_SIMP_TAC std_ss [bc_value_inv_def]));
-
-val update_ref_thm = store_thm("update_ref_thm",
-  ``abs_ml_inv (x::(RefPtr ptr)::stack) refs (roots,heap,a,sp) limit ==>
-    ?p r roots2 heap2.
-      (roots = r :: Pointer p :: roots2) /\
-      (heap_store p [RefBlock r] heap = (heap2,T)) /\
-      abs_ml_inv (x::(RefPtr ptr)::stack) (refs |+ (ptr,x)) (roots,heap2,a,sp) limit``,
-  SIMP_TAC std_ss [abs_ml_inv_def]
-  \\ REPEAT STRIP_TAC \\ FULL_SIMP_TAC std_ss [bc_stack_ref_inv_def]
-  \\ Cases_on `roots` \\ FULL_SIMP_TAC (srw_ss()) []
-  \\ Cases_on `t` \\ FULL_SIMP_TAC (srw_ss()) [bc_value_inv_def]
-  \\ `reachable_refs (x::RefPtr ptr::stack) refs ptr` by ALL_TAC THEN1
-   (FULL_SIMP_TAC std_ss [reachable_refs_def] \\ Q.EXISTS_TAC `RefPtr ptr`
-    \\ FULL_SIMP_TAC (srw_ss()) [get_refs_def])
-  \\ RES_TAC \\ POP_ASSUM MP_TAC \\ SIMP_TAC std_ss [Once bc_ref_inv_def]
-  \\ STRIP_TAC \\ FULL_SIMP_TAC std_ss []
-  \\ IMP_RES_TAC heap_store_RefBlock \\ POP_ASSUM (MP_TAC o SPEC_ALL)
-  \\ STRIP_TAC \\ FULL_SIMP_TAC std_ss []
-  \\ STRIP_TAC THEN1 (FULL_SIMP_TAC std_ss [roots_ok_def])
-  \\ STRIP_TAC THEN1
-   (FULL_SIMP_TAC std_ss [heap_ok_def] \\ REPEAT STRIP_TAC \\ RES_TAC THEN1
-     (POP_ASSUM MP_TAC \\ FULL_SIMP_TAC (srw_ss()) [RefBlock_def]
-      \\ ONCE_REWRITE_TAC [EQ_SYM_EQ] \\ REPEAT STRIP_TAC
-      \\ FULL_SIMP_TAC std_ss [roots_ok_def,MEM]) \\ RES_TAC)
-  \\ STRIP_TAC THEN1
-   (FULL_SIMP_TAC std_ss [unused_space_inv_def] \\ REPEAT STRIP_TAC
-    \\ RES_TAC \\ Cases_on `a = f ' ptr` \\ FULL_SIMP_TAC (srw_ss()) []
-    \\ FULL_SIMP_TAC (srw_ss()) [RefBlock_def])
-  \\ Q.EXISTS_TAC `f` \\ FULL_SIMP_TAC std_ss []
-  \\ FULL_SIMP_TAC std_ss []
-  \\ MP_TAC bc_value_inv_Ref
-  \\ FULL_SIMP_TAC std_ss [] \\ REPEAT STRIP_TAC
-  THEN1 (FULL_SIMP_TAC (srw_ss()) [SUBSET_DEF])
-  \\ Cases_on `n = ptr` \\ FULL_SIMP_TAC (srw_ss()) [bc_ref_inv_def]
-  THEN1 (Q.EXISTS_TAC `h` \\ FULL_SIMP_TAC std_ss [])
-  \\ FULL_SIMP_TAC std_ss [FAPPLY_FUPDATE_THM]
-  \\ `reachable_refs (x::RefPtr ptr::stack) refs n` by ALL_TAC
-  THEN1 IMP_RES_TAC reachable_refs_UPDATE \\ RES_TAC
-  \\ `f ' n <> f ' ptr` by ALL_TAC THEN1
-   (FULL_SIMP_TAC (srw_ss()) [INJ_DEF] \\ REPEAT STRIP_TAC \\ RES_TAC)
-  \\ RES_TAC \\ FULL_SIMP_TAC std_ss [] \\ FULL_SIMP_TAC (srw_ss()) [RefBlock_def]);
-
-(* new ref *)
-
-val new_ref_thm = store_thm("new_ref_thm",
-  ``abs_ml_inv (x::stack) refs (roots,heap,a,sp) limit /\
-    ~(ptr IN FDOM refs) /\ 2 <= sp ==>
-    ?p r roots2 heap2.
-      (roots = r :: roots2) /\
-      (heap_store_unused a sp (RefBlock r) heap = (heap2,T)) /\
-      abs_ml_inv (x::(RefPtr ptr)::stack) (refs |+ (ptr,x))
-                 (r::Pointer (a+sp-2)::roots2,heap2,a,sp-2) limit``,
-  SIMP_TAC std_ss [abs_ml_inv_def]
-  \\ REPEAT STRIP_TAC \\ FULL_SIMP_TAC std_ss [bc_stack_ref_inv_def]
-  \\ Cases_on `roots` \\ FULL_SIMP_TAC (srw_ss()) []
-  \\ `el_length (RefBlock h) <= sp` by ALL_TAC
-  THEN1 (FULL_SIMP_TAC std_ss [el_length_def,RefBlock_def])
-  \\ Q.PAT_ASSUM `unused_space_inv a sp heap` (fn th =>
-    MATCH_MP (IMP_heap_store_unused |> REWRITE_RULE [GSYM AND_IMP_INTRO] |> GEN_ALL) th
-    |> ASSUME_TAC)
-  \\ POP_ASSUM (MP_TAC o Q.SPEC `RefBlock h`) \\ MATCH_MP_TAC IMP_IMP
-  \\ STRIP_TAC THEN1 FULL_SIMP_TAC std_ss [RefBlock_def,el_length_def]
-  \\ STRIP_TAC \\ FULL_SIMP_TAC std_ss []
-  \\ `unused_space_inv a (sp - 2) heap2` by ALL_TAC
-  THEN1 FULL_SIMP_TAC std_ss [RefBlock_def,el_length_def]
-  \\ FULL_SIMP_TAC std_ss [] \\ STRIP_TAC THEN1
-   (FULL_SIMP_TAC std_ss [roots_ok_def,MEM,heap_store_rel_def] \\ REPEAT STRIP_TAC
-    \\ FULL_SIMP_TAC (srw_ss()) [RefBlock_def,el_length_def]
-    \\ FULL_SIMP_TAC (srw_ss()) [isSomeDataElement_def])
-  \\ STRIP_TAC THEN1
-   (FULL_SIMP_TAC std_ss [heap_ok_def,RefBlock_def,isForwardPointer_def]
-    \\ ONCE_REWRITE_TAC [EQ_SYM_EQ] \\ REPEAT STRIP_TAC THEN1
-     (POP_ASSUM MP_TAC \\ FULL_SIMP_TAC (srw_ss()) []
-      \\ ONCE_REWRITE_TAC [EQ_SYM_EQ] \\ REPEAT STRIP_TAC
-      \\ FULL_SIMP_TAC (srw_ss()) [roots_ok_def,MEM]
-      \\ METIS_TAC [heap_store_rel_def])
-    \\ RES_TAC \\ FULL_SIMP_TAC std_ss [heap_store_rel_def])
-  \\ `~(ptr IN FDOM f)` by (FULL_SIMP_TAC (srw_ss()) [SUBSET_DEF] \\ METIS_TAC [])
-  \\ Q.EXISTS_TAC `f |+ (ptr,a+sp-2)`
-  \\ STRIP_TAC THEN1
-   (FULL_SIMP_TAC (srw_ss()) [FDOM_FUPDATE]
-    \\ `(FAPPLY (f |+ (ptr,a + sp - 2))) = (ptr =+ (a+sp-2)) (FAPPLY f)` by
-     (FULL_SIMP_TAC std_ss [FUN_EQ_THM,FAPPLY_FUPDATE_THM,APPLY_UPDATE_THM]
-      \\ METIS_TAC []) \\ FULL_SIMP_TAC std_ss []
-    \\ MATCH_MP_TAC (METIS_PROVE [] ``!y. (x = y) /\ f y ==> f x``)
-    \\ Q.EXISTS_TAC `(a + sp - 2) INSERT {a | isSomeDataElement (heap_lookup a heap)}`
-    \\ STRIP_TAC
-    THEN1 (FULL_SIMP_TAC (srw_ss()) [RefBlock_def,isDataElement_def,el_length_def])
-    \\ MATCH_MP_TAC INJ_UPDATE \\ FULL_SIMP_TAC std_ss []
-    \\ FULL_SIMP_TAC (srw_ss()) []
-    \\ FULL_SIMP_TAC std_ss [RefBlock_def,el_length_def])
-  \\ STRIP_TAC THEN1
-     (FULL_SIMP_TAC (srw_ss()) [SUBSET_DEF,FDOM_FUPDATE] \\ METIS_TAC [])
-  \\ Q.ABBREV_TAC `f1 = f |+ (ptr,a + sp - 2)`
-  \\ `f SUBMAP f1` by ALL_TAC THEN1
-   (Q.UNABBREV_TAC `f1` \\ FULL_SIMP_TAC (srw_ss()) [SUBMAP_DEF,FAPPLY_FUPDATE_THM]
-    \\ METIS_TAC [])
-  \\ STRIP_TAC THEN1
-   (STRIP_TAC THEN1 METIS_TAC [bc_value_inv_SUBMAP] \\ STRIP_TAC THEN1
-     (Q.UNABBREV_TAC `f1`
-      \\ SIMP_TAC (srw_ss()) [bc_value_inv_def,FAPPLY_FUPDATE_THM,FDOM_FUPDATE])
-    \\ FULL_SIMP_TAC std_ss [EVERY2_EVERY,EVERY_MEM,MEM_ZIP,PULL_EXISTS]
-    \\ Q.PAT_ASSUM `LENGTH stack = LENGTH t` ASSUME_TAC
-    \\ FULL_SIMP_TAC std_ss [EVERY2_EVERY,EVERY_MEM,MEM_ZIP,PULL_EXISTS]
-    \\ REPEAT STRIP_TAC \\ METIS_TAC [bc_value_inv_SUBMAP])
-  \\ REPEAT STRIP_TAC
-  \\ Cases_on `n = ptr` THEN1
-   (Q.UNABBREV_TAC `f1` \\ ASM_SIMP_TAC (srw_ss()) [bc_ref_inv_def,FDOM_FUPDATE,
-      FAPPLY_FUPDATE_THM] \\ FULL_SIMP_TAC std_ss [el_length_def,RefBlock_def]
-    \\ SIMP_TAC (srw_ss()) [] \\ METIS_TAC [bc_value_inv_SUBMAP])
-  \\ `reachable_refs (x::RefPtr ptr::stack) refs n` by ALL_TAC
-  THEN1 IMP_RES_TAC reachable_refs_UPDATE
-  \\ Q.PAT_ASSUM `reachable_refs (x::RefPtr ptr::stack) (refs |+ (ptr,x)) n` (K ALL_TAC)
-  \\ `reachable_refs (x::stack) refs n` by ALL_TAC THEN1
-    (FULL_SIMP_TAC std_ss [reachable_refs_def] \\ REVERSE (Cases_on `x' = RefPtr ptr`)
-     THEN1 (FULL_SIMP_TAC std_ss [MEM] \\ METIS_TAC [])
-     \\ FULL_SIMP_TAC std_ss [get_refs_def,MEM]
-     \\ Q.PAT_ASSUM `RTC (ref_edge refs) r n` MP_TAC
-     \\ ONCE_REWRITE_TAC [RTC_CASES1]
-     \\ `r <> n` by FULL_SIMP_TAC std_ss [] \\ ASM_SIMP_TAC std_ss []
-     \\ FULL_SIMP_TAC std_ss [ref_edge_def])
-  \\ RES_TAC \\ Q.UNABBREV_TAC `f1` \\ FULL_SIMP_TAC std_ss [bc_ref_inv_def]
-  \\ ASM_SIMP_TAC (srw_ss()) [FDOM_FUPDATE,FAPPLY_FUPDATE_THM]
-  \\ `isSomeDataElement (heap_lookup (f ' n) heap)` by ALL_TAC THEN1
-    (FULL_SIMP_TAC std_ss [RefBlock_def] \\ EVAL_TAC \\ SIMP_TAC (srw_ss()) [])
-  \\ RES_TAC \\ FULL_SIMP_TAC std_ss [] \\ SIMP_TAC (srw_ss()) [RefBlock_def]
-  \\ FULL_SIMP_TAC std_ss [RefBlock_def] \\ IMP_RES_TAC heap_store_rel_lemma
-  \\ FULL_SIMP_TAC std_ss [] \\ SIMP_TAC (srw_ss()) []
-  \\ METIS_TAC [bc_value_inv_SUBMAP]);
-
-(* deref *)
-
-val heap_el_def = Define `
-  (heap_el (Pointer a) n heap =
-    case heap_lookup a heap of
-    | SOME (DataElement xs l d) =>
-        if n < LENGTH xs then (EL n xs,T) else (ARB,F)
-    | _ => (ARB,F)) /\
-  (heap_el _ _ _ = (ARB,F))`;
-
-val deref_thm = store_thm("deref_thm",
-  ``abs_ml_inv (RefPtr ptr::stack) refs (roots,heap,a,sp) limit ==>
-    ?r roots2 y.
-      (roots = r :: roots2) /\ (heap_el r 0 heap = (y,T)) /\ ptr IN FDOM refs /\
-      abs_ml_inv (refs ' ptr::RefPtr ptr::stack) refs (y::roots,heap,a,sp) limit``,
-  FULL_SIMP_TAC std_ss [abs_ml_inv_def,bc_stack_ref_inv_def]
-  \\ REPEAT STRIP_TAC \\ Cases_on `roots` \\ FULL_SIMP_TAC (srw_ss()) [EVERY2_def]
-  \\ FULL_SIMP_TAC std_ss [bc_value_inv_def]
-  \\ `reachable_refs (RefPtr ptr::stack) refs ptr` by ALL_TAC THEN1
-   (FULL_SIMP_TAC std_ss [reachable_refs_def,MEM] \\ Q.EXISTS_TAC `RefPtr ptr`
-    \\ ASM_SIMP_TAC (srw_ss()) [get_refs_def])
-  \\ RES_TAC \\ POP_ASSUM MP_TAC
-  \\ SIMP_TAC std_ss [Once bc_ref_inv_def] \\ REPEAT STRIP_TAC
-  \\ ASM_SIMP_TAC (srw_ss()) [heap_el_def,RefBlock_def]
-  \\ STRIP_TAC THEN1
-   (FULL_SIMP_TAC std_ss [roots_ok_def,heap_ok_def]
-    \\ IMP_RES_TAC heap_lookup_MEM
-    \\ STRIP_TAC \\ ONCE_REWRITE_TAC [MEM] \\ ONCE_REWRITE_TAC [EQ_SYM_EQ]
-    \\ REPEAT STRIP_TAC \\ RES_TAC
-    \\ FULL_SIMP_TAC std_ss [RefBlock_def]
-    \\ RES_TAC \\ FULL_SIMP_TAC std_ss [MEM])
-  \\ Q.EXISTS_TAC `f` \\ FULL_SIMP_TAC std_ss []
-  \\ REPEAT STRIP_TAC \\ Q.PAT_ASSUM `!xx.bbb` MATCH_MP_TAC
-  \\ Q.PAT_ASSUM `reachable_refs (RefPtr ptr::stack) refs ptr` (K ALL_TAC)
-  \\ FULL_SIMP_TAC std_ss [reachable_refs_def]
-  \\ REVERSE (Cases_on `x = refs ' ptr`)
-  THEN1 (FULL_SIMP_TAC std_ss [MEM] \\ METIS_TAC [])
-  \\ Q.EXISTS_TAC `RefPtr ptr` \\ SIMP_TAC std_ss [MEM,get_refs_def]
-  \\ ONCE_REWRITE_TAC [RTC_CASES1] \\ DISJ2_TAC
-  \\ Q.EXISTS_TAC `r` \\ FULL_SIMP_TAC std_ss []
-  \\ FULL_SIMP_TAC std_ss [ref_edge_def]);
-
-(* el *)
-
-val el_thm = store_thm("el_thm",
-  ``abs_ml_inv (Block n xs::stack) refs (roots,heap,a,sp) limit /\ i < LENGTH xs ==>
-    ?r roots2 y.
-      (roots = r :: roots2) /\ (heap_el r i heap = (y,T)) /\
-      abs_ml_inv (EL i xs::Block n xs::stack) refs (y::roots,heap,a,sp) limit``,
-  FULL_SIMP_TAC std_ss [abs_ml_inv_def,bc_stack_ref_inv_def]
-  \\ REPEAT STRIP_TAC \\ Cases_on `roots` \\ FULL_SIMP_TAC (srw_ss()) [EVERY2_def]
-  \\ FULL_SIMP_TAC std_ss [bc_value_inv_def]
-  \\ `xs <> []` by (REPEAT STRIP_TAC \\ FULL_SIMP_TAC std_ss [GSYM LENGTH_NIL,LENGTH])
-  \\ FULL_SIMP_TAC std_ss []
-  \\ ASM_SIMP_TAC (srw_ss()) [heap_el_def,BlockRep_def]
-  \\ IMP_RES_TAC EVERY2_LENGTH \\ FULL_SIMP_TAC std_ss []
-  \\ FULL_SIMP_TAC std_ss []
-  \\ STRIP_TAC THEN1
-   (FULL_SIMP_TAC std_ss [roots_ok_def,heap_ok_def] \\ ONCE_REWRITE_TAC [MEM]
-    \\ REPEAT STRIP_TAC \\ RES_TAC
-    \\ IMP_RES_TAC heap_lookup_MEM
-    \\ FULL_SIMP_TAC std_ss [BlockRep_def]
-    \\ `MEM (Pointer ptr') xs'` by ALL_TAC \\ RES_TAC
-    \\ FULL_SIMP_TAC std_ss [MEM_EL] \\ METIS_TAC [])
-  \\ Q.EXISTS_TAC `f` \\ FULL_SIMP_TAC std_ss []
-  \\ STRIP_TAC THEN1 (FULL_SIMP_TAC std_ss [EVERY2_EVERY,EVERY_MEM,MEM_ZIP,PULL_EXISTS])
-  \\ REPEAT STRIP_TAC
-  \\ Q.PAT_ASSUM `!xx.bbb` MATCH_MP_TAC
-  \\ FULL_SIMP_TAC std_ss [reachable_refs_def]
-  \\ REVERSE (Cases_on `x = EL i xs`)
-  THEN1 (FULL_SIMP_TAC std_ss [MEM] \\ METIS_TAC [])
-  \\ Q.LIST_EXISTS_TAC [`Block n xs`,`r`]
-  \\ ASM_SIMP_TAC std_ss [MEM]
-  \\ FULL_SIMP_TAC std_ss [get_refs_def,MEM_FLAT,MEM_MAP,PULL_EXISTS]
-  \\ Q.EXISTS_TAC `EL i xs` \\ FULL_SIMP_TAC std_ss []
-  \\ FULL_SIMP_TAC std_ss [MEM_EL] \\ Q.EXISTS_TAC `i`
-  \\ FULL_SIMP_TAC std_ss []);
-
-(* pop *)
-
-val pop_thm = store_thm("pop_thm",
-  ``abs_ml_inv (xs ++ stack) refs (rs ++ roots,heap,a,sp) limit /\
-    (LENGTH xs = LENGTH rs) ==>
-    abs_ml_inv (stack) refs (roots,heap,a,sp) limit``,
-  FULL_SIMP_TAC std_ss [abs_ml_inv_def,bc_stack_ref_inv_def] \\ REPEAT STRIP_TAC
-  \\ FULL_SIMP_TAC std_ss [roots_ok_def,MEM_APPEND]
-  \\ Q.EXISTS_TAC `f` \\ FULL_SIMP_TAC std_ss []
-  \\ IMP_RES_TAC EVERY2_APPEND \\ FULL_SIMP_TAC std_ss []
-  \\ REPEAT STRIP_TAC
-  \\ FULL_SIMP_TAC std_ss [reachable_refs_def,MEM_APPEND] \\ METIS_TAC []);
-
-(* permute stack *)
-
-val EVERY2_MAP_FST_SND = prove(
-  ``!xs. EVERY2 P (MAP FST xs) (MAP SND xs) = EVERY (\(x,y). P x y) xs``,
-  Induct \\ SRW_TAC [] [EVERY2_def] \\ Cases_on `h` \\ SRW_TAC [] []);
-
-val abs_ml_inv_stack_permute = store_thm("abs_ml_inv_stack_permute",
-  ``!xs ys.
-      abs_ml_inv (MAP FST xs ++ stack) refs (MAP SND xs ++ roots,heap,a,sp) limit /\
-      set ys SUBSET set xs ==>
-      abs_ml_inv (MAP FST ys ++ stack) refs (MAP SND ys ++ roots,heap,a,sp) limit``,
-  FULL_SIMP_TAC std_ss [abs_ml_inv_def,bc_stack_ref_inv_def] \\ REPEAT STRIP_TAC
-  \\ FULL_SIMP_TAC std_ss [roots_ok_def]
-  THEN1 (FULL_SIMP_TAC std_ss [MEM_APPEND,SUBSET_DEF,MEM_MAP] \\ METIS_TAC [])
-  \\ Q.EXISTS_TAC `f` \\ FULL_SIMP_TAC std_ss []
-  \\ FULL_SIMP_TAC std_ss [EVERY2_APPEND,LENGTH_MAP]
-  \\ FULL_SIMP_TAC std_ss [EVERY2_MAP_FST_SND]
-  \\ FULL_SIMP_TAC std_ss [EVERY_MEM,SUBSET_DEF]
-  \\ FULL_SIMP_TAC std_ss [reachable_refs_def,MEM_APPEND,MEM_MAP]
-  \\ METIS_TAC []);
-
-(* duplicate *)
-
-val duplicate_thm = store_thm("duplicate_thm",
-  ``abs_ml_inv (xs ++ stack) refs (rs ++ roots,heap,a,sp) limit /\
-    (LENGTH xs = LENGTH rs) ==>
-    abs_ml_inv (xs ++ xs ++ stack) refs (rs ++ rs ++ roots,heap,a,sp) limit``,
-  FULL_SIMP_TAC std_ss [abs_ml_inv_def,bc_stack_ref_inv_def] \\ REPEAT STRIP_TAC
-  \\ FULL_SIMP_TAC std_ss [roots_ok_def] THEN1 METIS_TAC [MEM_APPEND]
-  \\ Q.EXISTS_TAC `f` \\ FULL_SIMP_TAC std_ss []
-  \\ IMP_RES_TAC EVERY2_APPEND \\ FULL_SIMP_TAC std_ss []
-  \\ FULL_SIMP_TAC std_ss [APPEND_ASSOC]
-  \\ FULL_SIMP_TAC std_ss [reachable_refs_def,MEM_APPEND] \\ METIS_TAC []);
-
-val duplicate1_thm = save_thm("duplicate1_thm",
-  duplicate_thm |> Q.INST [`xs`|->`[x1]`,`rs`|->`[r1]`]
-                |> SIMP_RULE std_ss [LENGTH,APPEND]);
-
-(* move *)
-
-val IMP_EVERY2_APPEND = prove(
-  ``!xs1 ys1. EVERY2 P xs1 ys1 /\ EVERY2 P xs2 ys2 ==>
-              EVERY2 P (xs1 ++ xs2) (ys1 ++ ys2)``,
-  Induct \\ Cases_on `ys1` \\ FULL_SIMP_TAC (srw_ss()) [EVERY2_def] \\ METIS_TAC []);
-
-val EVERY2_APPEND_IMP = prove(
-  ``EVERY2 P (xs1 ++ xs2) (ys1 ++ ys2) ==>
-    (LENGTH xs1 = LENGTH ys1) ==> EVERY2 P xs1 ys1 /\ EVERY2 P xs2 ys2``,
-  REPEAT STRIP_TAC \\ IMP_RES_TAC EVERY2_LENGTH \\ IMP_RES_TAC EVERY2_APPEND);
-
-val move_thm = store_thm("move_thm",
-  ``!xs1 rs1 xs2 rs2 xs3 rs3.
-      abs_ml_inv (xs1 ++ xs2 ++ xs3 ++ stack) refs (rs1 ++ rs2 ++ rs3 ++ roots,heap,a,sp) limit /\
-      (LENGTH xs1 = LENGTH rs1) /\ (LENGTH xs2 = LENGTH rs2) /\ (LENGTH xs3 = LENGTH rs3) ==>
-      abs_ml_inv (xs1 ++ xs3 ++ xs2 ++ stack) refs (rs1 ++ rs3 ++ rs2 ++ roots,heap,a,sp) limit``,
-  REPEAT GEN_TAC
-  \\ FULL_SIMP_TAC std_ss [abs_ml_inv_def,bc_stack_ref_inv_def] \\ REPEAT STRIP_TAC
-  \\ FULL_SIMP_TAC std_ss [roots_ok_def] THEN1 METIS_TAC [MEM_APPEND]
-  \\ Q.EXISTS_TAC `f` \\ FULL_SIMP_TAC std_ss []
-  \\ STRIP_TAC THEN1
-   (NTAC 5 (IMP_RES_TAC EVERY2_APPEND_IMP \\ REPEAT (POP_ASSUM MP_TAC)
-    \\ FULL_SIMP_TAC std_ss [LENGTH_APPEND,AC ADD_COMM ADD_ASSOC]
-    \\ REPEAT STRIP_TAC)
-    \\ NTAC 5 (MATCH_MP_TAC IMP_EVERY2_APPEND \\ FULL_SIMP_TAC std_ss []))
-  \\ FULL_SIMP_TAC std_ss [reachable_refs_def,MEM_APPEND] \\ METIS_TAC []);
-
-(* splits *)
-
-val EVERY2_APPEND1 = prove(
-  ``!xs1 xs2 ys.
-      EVERY2 P (xs1 ++ xs2) ys ==>
-      ?ys1 ys2. (ys = ys1 ++ ys2) /\ (LENGTH xs1 = LENGTH ys1) /\ EVERY2 P xs2 ys2``,
-  Induct THEN1
-   (FULL_SIMP_TAC (srw_ss()) [] \\ REPEAT STRIP_TAC
-    \\ Q.EXISTS_TAC `[]` \\ FULL_SIMP_TAC (srw_ss()) [])
-  \\ Cases_on `ys` \\ FULL_SIMP_TAC (srw_ss()) [] \\ REPEAT STRIP_TAC
-  \\ RES_TAC \\ FULL_SIMP_TAC std_ss []
-  \\ Q.LIST_EXISTS_TAC [`h::ys1`,`ys2`] \\ FULL_SIMP_TAC (srw_ss()) []);
-
-val split1_thm = store_thm("split1_thm",
-  ``abs_ml_inv (xs1 ++ stack) refs (roots,heap,a,sp) limit ==>
-    ?rs1 roots1. (roots = rs1 ++ roots1) /\ (LENGTH rs1 = LENGTH xs1)``,
-  FULL_SIMP_TAC std_ss [abs_ml_inv_def,bc_stack_ref_inv_def,GSYM APPEND_ASSOC]
-  \\ REPEAT STRIP_TAC \\ NTAC 5 (IMP_RES_TAC EVERY2_APPEND1) \\ METIS_TAC []);
-
-val split2_thm = store_thm("split2_thm",
-  ``abs_ml_inv (xs1 ++ xs2 ++ stack) refs (roots,heap,a,sp) limit ==>
-    ?rs1 rs2 roots1. (roots = rs1 ++ rs2 ++ roots1) /\
-      (LENGTH rs1 = LENGTH xs1) /\ (LENGTH rs2 = LENGTH xs2)``,
-  FULL_SIMP_TAC std_ss [abs_ml_inv_def,bc_stack_ref_inv_def,GSYM APPEND_ASSOC]
-  \\ REPEAT STRIP_TAC \\ NTAC 5 (IMP_RES_TAC EVERY2_APPEND1) \\ METIS_TAC []);
-
-val split3_thm = store_thm("split3_thm",
-  ``abs_ml_inv (xs1 ++ xs2 ++ xs3 ++ stack) refs (roots,heap,a,sp) limit ==>
-    ?rs1 rs2 rs3 roots1. (roots = rs1 ++ rs2 ++ rs3 ++ roots1) /\
-      (LENGTH rs1 = LENGTH xs1) /\ (LENGTH rs2 = LENGTH xs2) /\
-      (LENGTH rs3 = LENGTH xs3)``,
-  FULL_SIMP_TAC std_ss [abs_ml_inv_def,bc_stack_ref_inv_def,GSYM APPEND_ASSOC]
-  \\ REPEAT STRIP_TAC \\ NTAC 5 (IMP_RES_TAC EVERY2_APPEND1) \\ METIS_TAC []);
-
-val LESS_EQ_LENGTH = store_thm("LESS_EQ_LENGTH",
-  ``!xs k. k <= LENGTH xs ==> ?ys1 ys2. (xs = ys1 ++ ys2) /\ (LENGTH ys1 = k)``,
-  Induct \\ Cases_on `k` \\ FULL_SIMP_TAC std_ss [LENGTH,ADD1,LENGTH_NIL,APPEND]
-  \\ REPEAT STRIP_TAC \\ RES_TAC \\ FULL_SIMP_TAC std_ss []
-  \\ Q.EXISTS_TAC `h::ys1` \\ FULL_SIMP_TAC std_ss [LENGTH,APPEND]
-  \\ SRW_TAC [] [ADD1]);
-
-val LESS_LENGTH = store_thm("LESS_LENGTH",
-  ``!xs k. k < LENGTH xs ==> ?ys1 y ys2. (xs = ys1 ++ y::ys2) /\ (LENGTH ys1 = k)``,
-  Induct \\ Cases_on `k` \\ FULL_SIMP_TAC std_ss [LENGTH,ADD1,LENGTH_NIL,APPEND]
-  \\ REPEAT STRIP_TAC \\ RES_TAC \\ FULL_SIMP_TAC std_ss [CONS_11]
-  \\ Q.EXISTS_TAC `h::ys1` \\ FULL_SIMP_TAC std_ss [LENGTH,APPEND]
-  \\ SRW_TAC [] [ADD1]);
 
 val _ = export_theory();
